books/projects/smtlink/verified/hint-interface.lisp
@@ -18,423 +18,423 @@
 ;;   :parents (verified)
 ;;   :short "Define default Smtlink hint interface"
 
-  (defprod hint-pair
-    :parents (smtlink-hint)
-    ((thm pseudo-termp "A theorem statement"
+(defprod hint-pair
+  :parents (smtlink-hint)
+  ((thm pseudo-termp "A theorem statement"
+        :default nil)
+   (hints true-listp "The ACL2 hint for proving this theorem"
           :default nil)
-     (hints true-listp "The ACL2 hint for proving this theorem"
-            :default nil)
-     (name symbolp "The name of the theorem if already proven in ACL2"
-           :default nil)))
+   (name symbolp "The name of the theorem if already proven in ACL2"
+         :default nil)))
 
-  (deflist hint-pair-list
-    :parents (hint-pair)
-    :elt-type hint-pair
-    :true-listp t)
+(deflist hint-pair-list
+  :parents (hint-pair)
+  :elt-type hint-pair
+  :true-listp t)
 
-  (defalist symbol-hint-pair-alist
-    :parents (hint-pair)
-    :key-type symbolp
-    :val-type hint-pair-p
-    :true-listp t)
+(defalist symbol-hint-pair-alist
+  :parents (hint-pair)
+  :key-type symbolp
+  :val-type hint-pair-p
+  :true-listp t)
 
-  (defprod decl
-    :parents (smtlink-hint)
-    ((name symbolp :default nil)
-     (type hint-pair-p :default (make-hint-pair))
-     ;; The fixer should be found in types;
-     ;; So we don't need fixer in function hints.
-     ;; (fixer symbolp :default nil)
-     ))
+(defprod decl
+  :parents (smtlink-hint)
+  ((name symbolp :default nil)
+   (type hint-pair-p :default (make-hint-pair))
+   ;; The fixer should be found in types;
+   ;; So we don't need fixer in function hints.
+   ;; (fixer symbolp :default nil)
+   ))
 
-  (deflist decl-list
-    :parents (decl)
-    :elt-type decl
-    :true-listp t)
+(deflist decl-list
+  :parents (decl)
+  :elt-type decl
+  :true-listp t)
 
-  (defprod smt-function
-    :parents (smtlink-hint)
-    ((name symbolp :default nil)
-     (expansion-depth natp :default 0)
-     (formals decl-list-p :default nil)
-     (returns decl-list-p :default nil)
-     ;; I'm not sure what's good of having guard,
-     ;; currently the hint is generated but is not used in Smtlink.
-     (guard hint-pair-p :default (make-hint-pair))
-     (more-returns hint-pair-list-p :default nil)))
+(defprod smt-function
+  :parents (smtlink-hint)
+  ((name symbolp :default nil)
+   (expansion-depth natp :default 0)
+   (formals decl-list-p :default nil)
+   (returns decl-list-p :default nil)
+   ;; I'm not sure what's good of having guard,
+   ;; currently the hint is generated but is not used in Smtlink.
+   (guard hint-pair-p :default (make-hint-pair))
+   (more-returns hint-pair-list-p :default nil)))
 
-  (defoption maybe-smt-function smt-function-p)
+(defoption maybe-smt-function smt-function-p)
 
-  (deflist smt-function-list
-    :parents (smt-function)
-    :elt-type smt-function-p
-    :true-listp t)
+(deflist smt-function-list
+  :parents (smt-function)
+  :elt-type smt-function-p
+  :true-listp t)
 
-  (defprod type-thm
-    ((name symbolp :default nil)
-     (hints true-listp :default nil)))
+(defprod type-thm
+  ((name symbolp :default nil)
+   (hints true-listp :default nil)))
 
-  (defprod type-function
-    ((name symbolp :default nil)
-     (return-type symbolp :default nil)
-     (type-of-function-thm type-thm-p :default (make-type-thm))
-     (destructor-of-constructor-thm type-thm-p :default (make-type-thm))
-     ;; constructor doesn't use this field
-     ))
+(defprod type-function
+  ((name symbolp :default nil)
+   (return-type symbolp :default nil)
+   (type-of-function-thm type-thm-p :default (make-type-thm))
+   (destructor-of-constructor-thm type-thm-p :default (make-type-thm))
+   ;; constructor doesn't use this field
+   ))
 
 (deflist type-function-list
   :parents (type-function)
   :elt-type type-function-p
   :true-listp t)
 
-  (defprod prod
-    ((kind symbolp :default nil)
-     (constructor type-function-p :default (make-type-function))
-     (destructors type-function-list-p :default nil)))
+(defprod prod
+  ((kind symbolp :default nil)
+   (constructor type-function-p :default (make-type-function))
+   (destructors type-function-list-p :default nil)))
 
-  (deflist prod-list
-    :elt-type prod-p
-    :true-listp t)
+(deflist prod-list
+  :elt-type prod-p
+  :true-listp t)
 
 (defalist symbol-prod-alist
   :key-type symbolp
   :val-type prod-p
   :true-listp t)
 
-  (deftagsum smt-type
-    (:abstract ())
-    (:array ((store type-function-p :default (make-type-function))
-             (select type-function-p :default (make-type-function))
-             (k type-function-p :default (make-type-function))
-             (key-type symbolp)
-             (val-type symbolp)
-             (array-thm type-thm-p :default (make-type-thm))))
-    ;; prod, list and option are all sums
-    (:sum ((kind-fn symbolp :default nil)
-           (prods prod-list-p :default nil)))
-    )
+(deftagsum smt-type
+  (:abstract ())
+  (:array ((store type-function-p :default (make-type-function))
+           (select type-function-p :default (make-type-function))
+           (k type-function-p :default (make-type-function))
+           (key-type symbolp)
+           (val-type symbolp)
+           (array-thm type-thm-p :default (make-type-thm))))
+  ;; prod, list and option are all sums
+  (:sum ((kind-fn symbolp :default nil)
+         (prods prod-list-p :default nil)))
+  )
 
-  (define smt-type-kind-fn ((smt-type smt-type-p))
-    :guard (equal (smt-type-kind smt-type) :sum)
-    (b* ((smt-type (smt-type-fix smt-type))
-         (kind-fn (smt-type-sum->kind-fn smt-type))
-         ((if (null kind-fn)) 'kind))
-      kind-fn))
+(define smt-type-kind-fn ((smt-type smt-type-p))
+  :guard (equal (smt-type-kind smt-type) :sum)
+  (b* ((smt-type (smt-type-fix smt-type))
+       (kind-fn (smt-type-sum->kind-fn smt-type))
+       ((if (null kind-fn)) 'kind))
+    kind-fn))
 
-  (defprod smt-fixtype
-    :parents (smtlink-hint)
-    ((name symbolp :default nil)
-     (recognizer symbolp :default nil)
-     (fixer symbolp :default nil)
-     (fixer-when-recognizer-thm type-thm-p :default (make-type-thm))
-     (basicp symbolp :default nil)
-     (kind smt-type-p :default (make-smt-type-abstract))))
+(defprod smt-fixtype
+  :parents (smtlink-hint)
+  ((name symbolp :default nil)
+   (recognizer symbolp :default nil)
+   (fixer symbolp :default nil)
+   (fixer-when-recognizer-thm type-thm-p :default (make-type-thm))
+   (basicp symbolp :default nil)
+   (kind smt-type-p :default (make-smt-type-abstract))))
 
-  (defoption maybe-smt-fixtype smt-fixtype-p)
+(defoption maybe-smt-fixtype smt-fixtype-p)
 
-  (deflist smt-fixtype-list
-    :parents (smt-fixtype)
-    :elt-type smt-fixtype-p
-    :true-listp t)
+(deflist smt-fixtype-list
+  :parents (smt-fixtype)
+  :elt-type smt-fixtype-p
+  :true-listp t)
 
-  (defprod info-pair
-    ((name symbolp)
-     (fn-type symbolp)
-     (kind symbolp))) ;; :store, :select, :recognizer, :fixer, :constructor,
-  ;; :destructor, :kind-fn
+(defprod info-pair
+  ((name symbolp)
+   (fn-type symbolp)
+   (kind symbolp))) ;; :store, :select, :recognizer, :fixer, :constructor,
+;; :destructor, :kind-fn
 
-  (defalist smt-fixtype-info
-    :key-type symbolp ;; function name
-    :val-type info-pair-p
-    :true-listp t)
+(defalist smt-fixtype-info
+  :key-type symbolp ;; function name
+  :val-type info-pair-p
+  :true-listp t)
 
-  (defprod smt-config
-    ((smt-cnf smtlink-config-p :default (make-smtlink-config))
-     (rm-file booleanp :default t)
-     (smt-dir stringp :default "")
-     (smt-fname stringp :default "")))
+(defprod smt-config
+  ((smt-cnf smtlink-config-p :default (make-smtlink-config))
+   (rm-file booleanp :default t)
+   (smt-dir stringp :default "")
+   (smt-fname stringp :default "")))
 
-  (deftagsum int-to-rat
-    (:switch ((okp booleanp :default nil)))
-    (:symbol-list ((lst symbol-listp :default nil))))
+(deftagsum int-to-rat
+  (:switch ((okp booleanp :default nil)))
+  (:symbol-list ((lst symbol-listp :default nil))))
 
-  (local (in-theory (disable symbol-listp)))
+(local (in-theory (disable symbol-listp)))
 
-  (defprod smtlink-hint
-    :parents (SMT-hint-interface)
-    ((functions smt-function-list-p :default nil)
-     (types smt-fixtype-list-p :default nil)
-     (types-info smt-fixtype-info-p :default nil)
-     (hypotheses hint-pair-list-p :default nil)
-     (configurations smt-config-p :default (make-smt-config))
+(defprod smtlink-hint
+  :parents (SMT-hint-interface)
+  ((functions smt-function-list-p :default nil)
+   (types smt-fixtype-list-p :default nil)
+   (types-info smt-fixtype-info-p :default nil)
+   (hypotheses hint-pair-list-p :default nil)
+   (configurations smt-config-p :default (make-smt-config))
 
-     (int-to-rat int-to-rat-p :default (make-int-to-rat-switch :okp nil))
-     (use-uninterpreted booleanp :default t)
-     (under-induct symbolp :default nil)
-     (global-hint symbolp :default nil)
-     (wrld-fn-len natp :default 0)
-     (custom-p booleanp :default nil)
-     ))
+   (int-to-rat int-to-rat-p :default (make-int-to-rat-switch :okp nil))
+   (use-uninterpreted booleanp :default t)
+   (under-induct symbolp :default nil)
+   (global-hint symbolp :default nil)
+   (wrld-fn-len natp :default 0)
+   (custom-p booleanp :default nil)
+   ))
 
-  (defalist smtlink-hint-alist
-    :key-type symbolp
-    :val-type smtlink-hint-p
-    :true-listp t)
+(defalist smtlink-hint-alist
+  :key-type symbolp
+  :val-type smtlink-hint-p
+  :true-listp t)
 
-  (defthm assoc-equal-of-smtlink-hint-alist
-    (implies (and (smtlink-hint-alist-p x)
-                  (consp (assoc-equal name x)))
-             (and (smtlink-hint-p (cdr (assoc-equal name x)))
-                  (cdr (assoc-equal name x)))))
-  ;; ---------------------------------------------------------------
-  ;; Utility functions
+(defthm assoc-equal-of-smtlink-hint-alist
+  (implies (and (smtlink-hint-alist-p x)
+                (consp (assoc-equal name x)))
+           (and (smtlink-hint-p (cdr (assoc-equal name x)))
+                (cdr (assoc-equal name x)))))
+;; ---------------------------------------------------------------
+;; Utility functions
 
-  ;; decl-list functions
-  (define get-thm-from-decl ((decl decl-p))
-    :returns (thm pseudo-termp)
-    (hint-pair->thm (decl->type (decl-fix decl))))
+;; decl-list functions
+(define get-thm-from-decl ((decl decl-p))
+  :returns (thm pseudo-termp)
+  (hint-pair->thm (decl->type (decl-fix decl))))
 
-  (define get-thms-from-decl-list ((dlst decl-list-p))
-    :returns (thms pseudo-term-listp)
-    :measure (len dlst)
-    (b* ((dlst (decl-list-fix dlst))
-         ((unless (consp dlst)) nil)
-         ((cons first rest) dlst))
-      (cons (get-thm-from-decl first)
-            (get-thms-from-decl-list rest))))
+(define get-thms-from-decl-list ((dlst decl-list-p))
+  :returns (thms pseudo-term-listp)
+  :measure (len dlst)
+  (b* ((dlst (decl-list-fix dlst))
+       ((unless (consp dlst)) nil)
+       ((cons first rest) dlst))
+    (cons (get-thm-from-decl first)
+          (get-thms-from-decl-list rest))))
 
-  ;; smt-function-list functions
-  (define is-function ((name symbolp) (fn-lst smt-function-list-p))
-    :returns (f maybe-smt-function-p)
-    :measure (len fn-lst)
-    (b* ((fn-lst (smt-function-list-fix fn-lst))
-         ((unless (consp fn-lst)) nil)
-         ((cons first rest) fn-lst)
-         (first-name (smt-function->name first))
-         ((if (equal first-name name)) first))
-      (is-function name rest)))
+;; smt-function-list functions
+(define is-function ((name symbolp) (fn-lst smt-function-list-p))
+  :returns (f maybe-smt-function-p)
+  :measure (len fn-lst)
+  (b* ((fn-lst (smt-function-list-fix fn-lst))
+       ((unless (consp fn-lst)) nil)
+       ((cons first rest) fn-lst)
+       (first-name (smt-function->name first))
+       ((if (equal first-name name)) first))
+    (is-function name rest)))
 
-  ;; smt-fixtype-list functions
-  (define generate-info-pair ((fn symbolp)
-                              (name symbolp)
-                              (fn-type symbolp)
-                              (kind symbolp)
-                              (acc smt-fixtype-info-p))
-    :returns (info smt-fixtype-info-p)
-    (b* ((fn (symbol-fix fn))
-         (name (symbol-fix name))
-         (kind (symbol-fix kind))
-         (fn-type (symbol-fix fn-type))
-         (acc (smt-fixtype-info-fix acc)))
-      (acons fn
-             (make-info-pair :name name
-                             :fn-type fn-type
-                             :kind kind)
-             acc)))
+;; smt-fixtype-list functions
+(define generate-info-pair ((fn symbolp)
+                            (name symbolp)
+                            (fn-type symbolp)
+                            (kind symbolp)
+                            (acc smt-fixtype-info-p))
+  :returns (info smt-fixtype-info-p)
+  (b* ((fn (symbol-fix fn))
+       (name (symbol-fix name))
+       (kind (symbol-fix kind))
+       (fn-type (symbol-fix fn-type))
+       (acc (smt-fixtype-info-fix acc)))
+    (acons fn
+           (make-info-pair :name name
+                           :fn-type fn-type
+                           :kind kind)
+           acc)))
 
-  (define generate-fixtype-info-array ((name symbolp)
-                                       (type smt-type-p)
-                                       (acc smt-fixtype-info-p))
-    :returns (info smt-fixtype-info-p)
-    :guard (equal (smt-type-kind type) :array)
-    (b* ((name (symbol-fix name))
-         (type (smt-type-fix type))
-         (acc (smt-fixtype-info-fix acc))
-         ((smt-type-array a) type)
-         (store-acc (generate-info-pair (type-function->name a.store)
-                                        name :store nil acc)))
-      (generate-info-pair (type-function->name a.select) name :select nil store-acc)))
-
-  (define generate-fixtype-info-destructors ((name symbolp)
-                                             (kind symbolp)
-                                             (destructors type-function-list-p)
-                                             (acc smt-fixtype-info-p))
-    :returns (info smt-fixtype-info-p)
-    :measure (len destructors)
-    (b* ((name (symbol-fix name))
-         (kind (symbol-fix kind))
-         (destructors (type-function-list-fix destructors))
-         (acc (smt-fixtype-info-fix acc))
-         ((unless (consp destructors)) acc)
-         ((cons first rest) destructors)
-         ((type-function f) first)
-         (first-acc (generate-info-pair f.name name :destructor kind acc)))
-      (generate-fixtype-info-destructors name kind rest first-acc)))
-
-  (define generate-fixtype-info-prod ((name symbolp)
-                                      (prod prod-p)
-                                      (acc smt-fixtype-info-p))
-    :returns (info smt-fixtype-info-p)
-    (b* ((name (symbol-fix name))
-         (prod (prod-fix prod))
-         ((prod p) prod)
-         (acc (smt-fixtype-info-fix acc))
-         (constructor-acc
-          (generate-info-pair (type-function->name p.constructor)
-                              name :constructor p.kind acc)))
-      (generate-fixtype-info-destructors name p.kind p.destructors
-                                         constructor-acc)))
-
-  (define generate-fixtype-info-prod-list ((name symbolp)
-                                           (prods prod-list-p)
-                                           (acc smt-fixtype-info-p))
-    :returns (info smt-fixtype-info-p)
-    :measure (len prods)
-    (b* ((name (symbol-fix name))
-         (prods (prod-list-fix prods))
-         (acc (smt-fixtype-info-fix acc))
-         ((unless (consp prods)) acc)
-         ((cons first rest) prods)
-         (first-acc (generate-fixtype-info-prod name first acc)))
-      (generate-fixtype-info-prod-list name rest first-acc)))
-
-  (define generate-fixtype-info-sum ((name symbolp)
+(define generate-fixtype-info-array ((name symbolp)
                                      (type smt-type-p)
                                      (acc smt-fixtype-info-p))
-    :returns (info smt-fixtype-info-p)
-    :guard (equal (smt-type-kind type) :sum)
-    (b* ((type (smt-type-fix type))
-         (acc (smt-fixtype-info-fix acc))
-         ((smt-type-sum s) type)
-         ((if (null s.kind-fn))
-          (generate-fixtype-info-prod-list name s.prods acc))
-         (new-acc (generate-info-pair s.kind-fn name :kind-fn nil acc)))
-      (generate-fixtype-info-prod-list name s.prods new-acc)))
+  :returns (info smt-fixtype-info-p)
+  :guard (equal (smt-type-kind type) :array)
+  (b* ((name (symbol-fix name))
+       (type (smt-type-fix type))
+       (acc (smt-fixtype-info-fix acc))
+       ((smt-type-array a) type)
+       (store-acc (generate-info-pair (type-function->name a.store)
+                                      name :store nil acc)))
+    (generate-info-pair (type-function->name a.select) name :select nil store-acc)))
 
-  (define generate-fixtype-info-kind ((name symbolp)
-                                      (type smt-type-p)
-                                      (acc smt-fixtype-info-p))
-    :returns (info smt-fixtype-info-p)
-    (b* ((type (smt-type-fix type))
-         (acc (smt-fixtype-info-fix acc))
-         (kind (smt-type-kind type)))
-      (case kind
-        (:array (generate-fixtype-info-array name type acc))
-        (:sum (generate-fixtype-info-sum name type acc))
-        (:abstract acc))))
+(define generate-fixtype-info-destructors ((name symbolp)
+                                           (kind symbolp)
+                                           (destructors type-function-list-p)
+                                           (acc smt-fixtype-info-p))
+  :returns (info smt-fixtype-info-p)
+  :measure (len destructors)
+  (b* ((name (symbol-fix name))
+       (kind (symbol-fix kind))
+       (destructors (type-function-list-fix destructors))
+       (acc (smt-fixtype-info-fix acc))
+       ((unless (consp destructors)) acc)
+       ((cons first rest) destructors)
+       ((type-function f) first)
+       (first-acc (generate-info-pair f.name name :destructor kind acc)))
+    (generate-fixtype-info-destructors name kind rest first-acc)))
 
-  (define generate-one-fixtype-info ((type smt-fixtype-p)
-                                     (acc smt-fixtype-info-p))
-    :returns (info smt-fixtype-info-p)
-    (b* ((type (smt-fixtype-fix type))
-         (acc (smt-fixtype-info-fix acc))
-         ((smt-fixtype f) type)
-         (rec-acc (generate-info-pair f.recognizer f.name :recognizer nil acc))
-         (fix-acc (generate-info-pair f.fixer f.name :fixer nil rec-acc)))
-      (generate-fixtype-info-kind f.name f.kind fix-acc)))
+(define generate-fixtype-info-prod ((name symbolp)
+                                    (prod prod-p)
+                                    (acc smt-fixtype-info-p))
+  :returns (info smt-fixtype-info-p)
+  (b* ((name (symbol-fix name))
+       (prod (prod-fix prod))
+       ((prod p) prod)
+       (acc (smt-fixtype-info-fix acc))
+       (constructor-acc
+        (generate-info-pair (type-function->name p.constructor)
+                            name :constructor p.kind acc)))
+    (generate-fixtype-info-destructors name p.kind p.destructors
+                                       constructor-acc)))
 
-  (define generate-fixtype-info ((types smt-fixtype-list-p)
-                                 (acc smt-fixtype-info-p))
-    :returns (info smt-fixtype-info-p)
-    :measure (len types)
-    (b* ((types (smt-fixtype-list-fix types))
-         (acc (smt-fixtype-info-fix acc))
-         ((unless (consp types)) acc)
-         ((cons first rest) types)
-         (new-acc (generate-one-fixtype-info first acc)))
-      (generate-fixtype-info rest new-acc)))
+(define generate-fixtype-info-prod-list ((name symbolp)
+                                         (prods prod-list-p)
+                                         (acc smt-fixtype-info-p))
+  :returns (info smt-fixtype-info-p)
+  :measure (len prods)
+  (b* ((name (symbol-fix name))
+       (prods (prod-list-fix prods))
+       (acc (smt-fixtype-info-fix acc))
+       ((unless (consp prods)) acc)
+       ((cons first rest) prods)
+       (first-acc (generate-fixtype-info-prod name first acc)))
+    (generate-fixtype-info-prod-list name rest first-acc)))
 
-  (define add-fixtype-info ((hint smtlink-hint-p))
-    :returns (new-hint smtlink-hint-p)
-    (b* ((hint (smtlink-hint-fix hint))
-         ((smtlink-hint h) hint)
-         (info (generate-fixtype-info h.types nil)))
-      (change-smtlink-hint hint :types-info info)))
+(define generate-fixtype-info-sum ((name symbolp)
+                                   (type smt-type-p)
+                                   (acc smt-fixtype-info-p))
+  :returns (info smt-fixtype-info-p)
+  :guard (equal (smt-type-kind type) :sum)
+  (b* ((type (smt-type-fix type))
+       (acc (smt-fixtype-info-fix acc))
+       ((smt-type-sum s) type)
+       ((if (null s.kind-fn))
+        (generate-fixtype-info-prod-list name s.prods acc))
+       (new-acc (generate-info-pair s.kind-fn name :kind-fn nil acc)))
+    (generate-fixtype-info-prod-list name s.prods new-acc)))
 
-  (define is-type ((x symbolp) (fixtypes smt-fixtype-list-p))
-    :returns (type maybe-smt-fixtype-p)
-    :measure (len fixtypes)
-    (b* ((fixtypes (smt-fixtype-list-fix fixtypes))
-         ((unless (consp fixtypes)) nil)
-         ((cons first rest) fixtypes)
-         ((if (equal x (smt-fixtype->recognizer first))) first))
-      (is-type x rest)))
+(define generate-fixtype-info-kind ((name symbolp)
+                                    (type smt-type-p)
+                                    (acc smt-fixtype-info-p))
+  :returns (info smt-fixtype-info-p)
+  (b* ((type (smt-type-fix type))
+       (acc (smt-fixtype-info-fix acc))
+       (kind (smt-type-kind type)))
+    (case kind
+      (:array (generate-fixtype-info-array name type acc))
+      (:sum (generate-fixtype-info-sum name type acc))
+      (:abstract acc))))
 
-  (define is-recognizer ((x symbolp) (fixinfo smt-fixtype-info-p))
-    :returns (okp booleanp)
-    (b* ((fixinfo (smt-fixtype-info-fix fixinfo))
-         (item (assoc-equal x fixinfo))
-         ((unless item) nil)
-         ((info-pair p) (cdr item)))
-      (equal p.fn-type :recognizer)))
+(define generate-one-fixtype-info ((type smt-fixtype-p)
+                                   (acc smt-fixtype-info-p))
+  :returns (info smt-fixtype-info-p)
+  (b* ((type (smt-fixtype-fix type))
+       (acc (smt-fixtype-info-fix acc))
+       ((smt-fixtype f) type)
+       (rec-acc (generate-info-pair f.recognizer f.name :recognizer nil acc))
+       (fix-acc (generate-info-pair f.fixer f.name :fixer nil rec-acc)))
+    (generate-fixtype-info-kind f.name f.kind fix-acc)))
 
-  (define is-fixer ((x symbolp) (fixinfo smt-fixtype-info-p))
-    :returns (okp booleanp)
-    (b* ((fixinfo (smt-fixtype-info-fix fixinfo))
-         (item (assoc-equal x fixinfo))
-         ((unless item) nil)
-         ((info-pair p) (cdr item)))
-      (equal p.fn-type :fixer)))
+(define generate-fixtype-info ((types smt-fixtype-list-p)
+                               (acc smt-fixtype-info-p))
+  :returns (info smt-fixtype-info-p)
+  :measure (len types)
+  (b* ((types (smt-fixtype-list-fix types))
+       (acc (smt-fixtype-info-fix acc))
+       ((unless (consp types)) acc)
+       ((cons first rest) types)
+       (new-acc (generate-one-fixtype-info first acc)))
+    (generate-fixtype-info rest new-acc)))
 
-  (define name-of-recognizer ((x symbolp) (fixinfo smt-fixtype-info-p))
-    :returns (name symbolp)
-    (b* ((fixinfo (smt-fixtype-info-fix fixinfo))
-         (item (assoc-equal x fixinfo))
-         ((unless item) nil)
-         ((info-pair p) (cdr item)))
-      p.name))
+(define add-fixtype-info ((hint smtlink-hint-p))
+  :returns (new-hint smtlink-hint-p)
+  (b* ((hint (smtlink-hint-fix hint))
+       ((smtlink-hint h) hint)
+       (info (generate-fixtype-info h.types nil)))
+    (change-smtlink-hint hint :types-info info)))
 
-  (define fncall-of-fixtypes ((x symbolp) (fixinfo smt-fixtype-info-p))
-    :returns (ok booleanp)
-    (b* ((fixinfo (smt-fixtype-info-fix fixinfo)))
-      (not (null (assoc-equal x fixinfo)))))
+(define is-type ((x symbolp) (fixtypes smt-fixtype-list-p))
+  :returns (type maybe-smt-fixtype-p)
+  :measure (len fixtypes)
+  (b* ((fixtypes (smt-fixtype-list-fix fixtypes))
+       ((unless (consp fixtypes)) nil)
+       ((cons first rest) fixtypes)
+       ((if (equal x (smt-fixtype->recognizer first))) first))
+    (is-type x rest)))
 
-  (define fixer-of-recognizer ((x symbolp) (fixtypes smt-fixtype-list-p))
-    :returns (fixer symbolp)
-    :measure (len fixtypes)
-    (b* ((fixtypes (smt-fixtype-list-fix fixtypes))
-         ((unless (consp fixtypes)) nil)
-         ((cons first rest) fixtypes)
-         ((if (equal x (smt-fixtype->recognizer first)))
-          (smt-fixtype->fixer first)))
-      (fixer-of-recognizer x rest)))
+(define is-recognizer ((x symbolp) (fixinfo smt-fixtype-info-p))
+  :returns (okp booleanp)
+  (b* ((fixinfo (smt-fixtype-info-fix fixinfo))
+       (item (assoc-equal x fixinfo))
+       ((unless item) nil)
+       ((info-pair p) (cdr item)))
+    (equal p.fn-type :recognizer)))
 
-  (define recognizer-of-fixer ((x symbolp) (fixtypes smt-fixtype-list-p))
-    :returns (recognizer symbolp)
-    :measure (len fixtypes)
-    (b* ((fixtypes (smt-fixtype-list-fix fixtypes))
-         ((unless (consp fixtypes)) nil)
-         ((cons first rest) fixtypes)
-         ((if (equal x (smt-fixtype->fixer first)))
-          (smt-fixtype->recognizer first)))
-      (recognizer-of-fixer x rest)))
+(define is-fixer ((x symbolp) (fixinfo smt-fixtype-info-p))
+  :returns (okp booleanp)
+  (b* ((fixinfo (smt-fixtype-info-fix fixinfo))
+       (item (assoc-equal x fixinfo))
+       ((unless item) nil)
+       ((info-pair p) (cdr item)))
+    (equal p.fn-type :fixer)))
 
-  (define type-decl-p ((expr pseudo-termp)
-                       (fixinfo smt-fixtype-info-p))
-    :returns (is-decl? booleanp)
-    (b* (;; ((if (is-type-hyp-decl expr)) t)
-         ((unless (equal (len expr) 2))
-          nil)
-         (fn-name (car expr))
-         ((unless (symbolp fn-name)) nil)
-         ((unless (is-recognizer fn-name fixinfo))
-          nil)
-         ((unless (and (symbolp (cadr expr)) (cadr expr))) nil))
-      t)
-    ///
-    (more-returns
-     (is-decl?
-      (implies is-decl?
-               (and (consp expr)
-                    (consp (cdr expr))
-                    (symbolp (car expr))
-                    (is-recognizer (car expr) fixinfo)
-                    (symbolp (cadr expr)) (cadr expr)))
-      :name type-decl-p-definition)))
+(define name-of-recognizer ((x symbolp) (fixinfo smt-fixtype-info-p))
+  :returns (name symbolp)
+  (b* ((fixinfo (smt-fixtype-info-fix fixinfo))
+       (item (assoc-equal x fixinfo))
+       ((unless item) nil)
+       ((info-pair p) (cdr item)))
+    p.name))
 
-  (define return-type-of-function ((f smt-function-p)
-                                   (fixinfo smt-fixtype-info-p))
-    :returns (type symbolp)
-    (b* ((f (smt-function-fix f))
-         ((smt-function f) f)
-         ((unless (and (consp f.returns)
-                       (null (cdr f.returns))))
-          (er hard? 'hint-interface=>return-type-of-function
-              "Smtlink only supports functions that return one value, but ~p0
+(define fncall-of-fixtypes ((x symbolp) (fixinfo smt-fixtype-info-p))
+  :returns (ok booleanp)
+  (b* ((fixinfo (smt-fixtype-info-fix fixinfo)))
+    (not (null (assoc-equal x fixinfo)))))
+
+(define fixer-of-recognizer ((x symbolp) (fixtypes smt-fixtype-list-p))
+  :returns (fixer symbolp)
+  :measure (len fixtypes)
+  (b* ((fixtypes (smt-fixtype-list-fix fixtypes))
+       ((unless (consp fixtypes)) nil)
+       ((cons first rest) fixtypes)
+       ((if (equal x (smt-fixtype->recognizer first)))
+        (smt-fixtype->fixer first)))
+    (fixer-of-recognizer x rest)))
+
+(define recognizer-of-fixer ((x symbolp) (fixtypes smt-fixtype-list-p))
+  :returns (recognizer symbolp)
+  :measure (len fixtypes)
+  (b* ((fixtypes (smt-fixtype-list-fix fixtypes))
+       ((unless (consp fixtypes)) nil)
+       ((cons first rest) fixtypes)
+       ((if (equal x (smt-fixtype->fixer first)))
+        (smt-fixtype->recognizer first)))
+    (recognizer-of-fixer x rest)))
+
+(define type-decl-p ((expr pseudo-termp)
+                     (fixinfo smt-fixtype-info-p))
+  :returns (is-decl? booleanp)
+  (b* (;; ((if (is-type-hyp-decl expr)) t)
+       ((unless (equal (len expr) 2))
+        nil)
+       (fn-name (car expr))
+       ((unless (symbolp fn-name)) nil)
+       ((unless (is-recognizer fn-name fixinfo))
+        nil)
+       ((unless (and (symbolp (cadr expr)) (cadr expr))) nil))
+    t)
+  ///
+  (more-returns
+   (is-decl?
+    (implies is-decl?
+             (and (consp expr)
+                  (consp (cdr expr))
+                  (symbolp (car expr))
+                  (is-recognizer (car expr) fixinfo)
+                  (symbolp (cadr expr)) (cadr expr)))
+    :name type-decl-p-definition)))
+
+(define return-type-of-function ((f smt-function-p)
+                                 (fixinfo smt-fixtype-info-p))
+  :returns (type symbolp)
+  (b* ((f (smt-function-fix f))
+       ((smt-function f) f)
+       ((unless (and (consp f.returns)
+                     (null (cdr f.returns))))
+        (er hard? 'hint-interface=>return-type-of-function
+            "Smtlink only supports functions that return one value, but ~p0
     returns two: ~p1~%" f.name f.returns))
-         (type-thm (hint-pair->thm (decl->type (car f.returns))))
-         ((unless (type-decl-p type-thm fixinfo))
-          (er hard? 'hint-interface=>return-type-of-function
-              "Not a type declaration: ~p0~%" type-thm)))
-      (car type-thm)))
+       (type-thm (hint-pair->thm (decl->type (car f.returns))))
+       ((unless (type-decl-p type-thm fixinfo))
+        (er hard? 'hint-interface=>return-type-of-function
+            "Not a type declaration: ~p0~%" type-thm)))
+    (car type-thm)))
 ;;  )
