books/projects/smtlink/verified/reorder-hypotheses.lisp
@@ -1,0 +1,272 @@
+;; Copyright (C) 2015, University of British Columbia
+;; Written by Yan Peng (March 3rd 2021)
+;;
+;; License: A 3-clause BSD license.
+;; See the LICENSE file distributed with ACL2
+;;
+
+(in-package "SMT")
+(include-book "std/util/bstar" :dir :system)
+(include-book "xdoc/top" :dir :system)
+(include-book "std/util/define" :dir :system)
+(include-book "centaur/fty/top" :dir :system)
+
+(include-book "extractor")
+
+(define filter-type-hypo ((hypo-lst pseudo-term-listp)
+                          (fixinfo smt-fixtype-info-p))
+  :returns (mv (root-hypo pseudo-term-listp)
+               (rest-hypo pseudo-term-listp))
+  (b* ((hypo-lst (pseudo-term-list-fix hypo-lst))
+       (fixinfo (smt-fixtype-info-fix fixinfo))
+       ((unless (consp hypo-lst)) (mv nil nil))
+       ((cons hypo-hd hypo-tl) hypo-lst)
+       ((mv tl-root tl-rest) (filter-type-hypo hypo-tl fixinfo))
+       ((if (type-decl-p hypo-hd fixinfo))
+        (mv (cons hypo-hd tl-root) tl-rest)))
+    (mv tl-root (cons hypo-hd tl-rest))))
+
+#|
+(filter-type-hypo '((equal x2 (binary-+ x0 x1))
+                    (equal x1 (rfix y))
+                    (equal x0 (ifix x))
+                    (integerp x)
+                    (rationalp y))
+                  `((integerp . ,(make-info-pair :fn-type :recognizer))
+                    (rationalp . ,(make-info-pair :fn-type :recognizer))))
+|#
+
+(defalist pseudo-term-symbol-list-alist
+  :key-type pseudo-termp
+  :val-type symbol-listp
+  :true-listp t
+  :pred pseudo-term-symbol-list-alistp)
+
+(defthm symbol-list-of-simple-term-vars
+  (symbol-listp (acl2::simple-term-vars term)))
+
+(acl2::make-flag flag-merge-sort-lexorder
+                 acl2::merge-sort-lexorder
+                 :flag-mapping ((pseudo-termp     . term)
+                                (pseudo-term-listp . lst))
+                 :defthm-macro-name defthm-flag-pseudo-termp
+                 :flag-var flag)
+
+(defthm symbol-list-of-merge-lexorder
+  (implies (and (symbol-listp l1)
+                (symbol-listp l2)
+                (symbol-listp acc))
+           (symbol-listp (acl2::merge-lexorder l1 l2 acc))))
+
+(defthm symbol-list-of-evens
+  (implies (symbol-listp l) (symbol-listp (evens l)))
+  :hints (("Goal" :induct (evens l))))
+
+(defthm symbol-list-of-merge-sort-lexorder
+  (implies (symbol-listp x)
+           (symbol-listp (acl2::merge-sort-lexorder x))))
+
+(define make-nodes ((hypo-lst pseudo-term-listp)
+                    (acc pseudo-term-symbol-list-alistp))
+  :returns (branches pseudo-term-symbol-list-alistp)
+  (b* ((hypo-lst (pseudo-term-list-fix hypo-lst))
+       (acc (pseudo-term-symbol-list-alist-fix acc))
+       ((unless (consp hypo-lst)) acc)
+       ((cons hypo-hd hypo-tl) hypo-lst)
+       ((mv okp term) (case-match hypo-hd
+                        (('equal & term) (mv t term))
+                        (& (mv nil nil))))
+       ((unless okp)
+        (er hard? 'reorder-hypotheses=>make-nodes "bad equality: ~q0" hypo-hd))
+       (free-vars (acl2::merge-sort-lexorder (acl2::simple-term-vars term)))
+       (exist? (assoc-equal term acc))
+       ((if exist?) (make-nodes hypo-tl acc)))
+    (make-nodes hypo-tl (acons hypo-hd free-vars acc))))
+
+#|
+(make-nodes '((equal x2 (binary-+ x0 x1))
+              (equal x1 (rfix y))
+              (equal x0 (ifix x))
+              (equal x3 (ifix x)))
+            nil)
+|#
+
+(define update-roots ((node-alist pseudo-term-symbol-list-alistp)
+                      (roots symbol-listp)
+                      (sorted pseudo-term-listp))
+  :returns (mv (new-roots symbol-listp)
+               (new-sorted pseudo-term-listp))
+  :measure (len (pseudo-term-symbol-list-alist-fix node-alist))
+  (b* ((node-alist (pseudo-term-symbol-list-alist-fix node-alist))
+       (roots (symbol-list-fix roots))
+       (sorted (pseudo-term-list-fix sorted))
+       ((unless (consp node-alist)) (mv roots sorted))
+       ((cons node-hd node-tl) node-alist)
+       ((cons equality var-lst) node-hd)
+       ((if (or (member-equal equality sorted)
+                (not (subsetp-equal var-lst roots))))
+        (update-roots node-tl roots sorted))
+       ((mv okp new-var)
+        (case-match equality
+          (('equal new-var &) (mv t new-var))
+          (& (mv nil nil))))
+       ((unless (and okp (symbolp new-var)))
+        (prog2$ (er hard? 'reorder-hypotheses=>update-roots
+                    "bad equality: ~q0" equality)
+                (mv roots sorted))))
+    (update-roots node-tl (cons new-var roots) (cons equality sorted)))
+  ///
+  (more-returns
+   (new-sorted (implies (pseudo-term-listp sorted)
+                        (>= (len new-sorted)
+                            (len sorted)))
+               :name update-roots-nondecrease-len-of-sorted)
+   (new-sorted (implies (and (pseudo-term-listp sorted)
+                             (not (equal new-sorted sorted)))
+                        (> (len new-sorted)
+                           (len sorted)))
+               :name update-roots-increase-len-of-sorted)))
+
+#|
+(update-roots '(((equal x2 (binary-+ x0 x1)) x0 x1)
+                ((equal x3 (ifix x)) x)
+                ((equal x0 (ifix x)) x)
+                ((equal x1 (rfix y)) y))
+              '(x y)
+              nil)
+
+(update-roots '(((equal x2 (binary-+ x0 x1)) x0 x1)
+                ((equal x3 (ifix x)) x)
+                ((equal x0 (ifix x)) x)
+                ((equal x1 (rfix y)) y))
+              '(x1 x0 x3 x y)
+              '((equal x1 (rfix y))
+                (equal x0 (ifix x))
+                (equal x3 (ifix x))))
+|#
+
+(define measure-of-order-equality-hypo
+  ((node-alist pseudo-term-symbol-list-alistp)
+   (sorted pseudo-term-listp))
+  :returns (m natp)
+  (if (< (len (pseudo-term-list-fix sorted))
+         (len (pseudo-term-symbol-list-alist-fix node-alist)))
+      (- (len (pseudo-term-symbol-list-alist-fix node-alist))
+         (len (pseudo-term-list-fix sorted)))
+    0))
+
+(define order-equality-hypo ((node-alist pseudo-term-symbol-list-alistp)
+                             (roots symbol-listp)
+                             (sorted pseudo-term-listp))
+  :returns (mv (new-roots symbol-listp)
+               (new-sorted pseudo-term-listp))
+  :measure (measure-of-order-equality-hypo node-alist sorted)
+  :hints (("Goal"
+           :in-theory (e/d (measure-of-order-equality-hypo)
+                           (update-roots-increase-len-of-sorted))
+           :use ((:instance update-roots-increase-len-of-sorted
+                            (node-alist (pseudo-term-symbol-list-alist-fix node-alist))
+                            (roots (symbol-list-fix roots))
+                            (sorted (pseudo-term-list-fix sorted))))))
+  (b* ((node-alist (pseudo-term-symbol-list-alist-fix node-alist))
+       (roots (symbol-list-fix roots))
+       (sorted (pseudo-term-list-fix sorted))
+       ((if (>= (len sorted) (len node-alist))) (mv roots sorted))
+       ((mv new-roots new-sorted) (update-roots node-alist roots sorted))
+       ((if (equal new-sorted sorted)) (mv new-roots new-sorted)))
+    (order-equality-hypo node-alist new-roots new-sorted)))
+
+(define initialize-roots ((type-hypo pseudo-term-listp))
+  :returns (roots symbol-listp)
+  (b* ((type-hypo (pseudo-term-list-fix type-hypo))
+       ((unless (consp type-hypo)) nil)
+       ((cons hypo-hd hypo-tl) type-hypo)
+       ((mv okp var) (case-match hypo-hd
+                       ((& var) (mv t var))
+                       (& (mv nil nil))))
+       ((unless (and okp (symbolp var)))
+        (prog2$ (er hard? 'reorder-hypotheses=>initialize-roots
+                    "bad type hypotheses: ~q0" hypo-hd)
+                nil)))
+    (cons var (initialize-roots hypo-tl))))
+
+(defthm pseudo-term-list-of-rev
+  (implies (pseudo-term-listp x)
+           (pseudo-term-listp (acl2::rev x)))
+  :hints (("Goal"
+           :in-theory (enable acl2::rev)
+           :induct (acl2::rev x))))
+
+(defthm pseudo-term-list-of-reverse
+  (implies (pseudo-term-listp x)
+           (pseudo-term-listp (reverse x))))
+
+(define order-hypo-lst ((hypo-lst pseudo-term-listp)
+                        (fixinfo smt-fixtype-info-p))
+  :returns (new-hypo-lst pseudo-term-listp
+                         :hints (("Goal" :in-theory (disable reverse))))
+  (b* ((hypo-lst (pseudo-term-list-fix hypo-lst))
+       (fixinfo (smt-fixtype-info-fix fixinfo))
+       ((mv root-hypo rest-hypo) (filter-type-hypo hypo-lst fixinfo))
+       (node-alist (make-nodes rest-hypo nil))
+       (roots (initialize-roots root-hypo))
+       ((mv & ordered-rest)
+        (order-equality-hypo node-alist roots nil))
+       ((if (< (len ordered-rest) (len node-alist)))
+        (prog2$ (er hard? 'reorder-hypotheses=>order-hypo-lst
+                    "Can't order hypotheses: ~q0" rest-hypo)
+                hypo-lst)))
+    (append root-hypo (reverse ordered-rest))))
+
+#|
+(order-hypo-lst '((equal x2 (binary-+ x0 x1))
+                  (equal x4 (unary-- x1))
+                  (equal x3 (binary-* x0 x2))
+                  (equal x1 (rfix y))
+                  (equal x0 (ifix x))
+                  (rationalp y)
+                  (integerp x))
+                `((integerp . ,(make-info-pair :fn-type :recognizer))
+                  (rationalp . ,(make-info-pair :fn-type :recognizer))))
+|#
+
+stop
+
+(defthm correctness-of-order-hypo-lst
+  (implies (and (pseudo-term-listp hypo-lst)
+                (smt-fixtype-info-p fixinfo)
+                (alistp a))
+           (equal (ev-smtcp-lst (order-hypo-lst hypo-lst fixinfo) a)
+                  (ev-smtcp-lst hypo-lst a)))
+  :hints (("Goal"
+           :in-theory (enable order-hypo-lst))))
+
+(defthm correctness-of-order-hypo-lst-corollary
+  (implies (and (pseudo-term-listp hypo-lst)
+                (alistp a))
+           (equal (ev-smtcp (conjoin (order-hypo-lst hypo-lst)) a)
+                  (ev-smtcp (conjoin hypo-lst) a)))
+  :hints (("Goal"
+           :in-theory (enable order-hypo-lst))))
+
+(define reorder-hypotheses ((term pseudo-termp)
+                            (hint smtlink-hint-p))
+  :returns (new-term pseudo-termp)
+  (b* ((term (pseudo-term-fix term))
+       (hint (smtlink-hint-fix hint))
+       ((smtlink-hint h) hint)
+       ((mv hypo-lst new-term) (extractor term h.types-info))
+       (ordered-hypo (order-hypo-lst hypo-lst h.types-info)))
+    `(if ,(conjoin ordered-hypo) ,new-term 't)))
+
+(defthm correctness-of-reorder-hypotheses
+  (implies (and (pseudo-termp term)
+                (smtlink-hint-p hint)
+                (alistp a)
+                (ev-smtcp (reorder-hypotheses term hint) a))
+           (ev-smtcp term a))
+  :hints (("Goal"
+           :in-theory (e/d (reorder-hypotheses)
+                           (correctness-of-extractor))
+           :use ((:instance correctness-of-extractor
+                            (fixinfo (smtlink-hint->types-info hint)))))))
