books/projects/smtlink/verified/test/test-expand.lisp
@@ -1,0 +1,36 @@
+(in-package "SMT")
+(ld "../expand-cp.lisp")
+(ld "test-smtlink-hint.lisp")
+
+(set-guard-checking :none)
+
+(defun term ()
+  '(if (if (integerp x)
+           (rationalp y)
+         'nil)
+       (< (foo x y) '0)
+     't)
+  )
+
+(expand-cp (list (term)) (my-hint) state)
+
+(defun term2 ()
+  '(if (if (integerp x)
+           (rationalp y)
+         'nil)
+       (< ((lambda (a b) (binary-+ a b)) x y) '0)
+     't))
+
+(expand-cp (list (term2)) (my-hint) state)
+
+(defun term3 ()
+  '(if (if (< x y)
+           (if (integerp x)
+               (rationalp y)
+             'nil)
+         'nil)
+       (< (foo x y) '0)
+     't)
+  )
+
+(expand-cp (list (term3)) (my-hint) state)
