books/projects/smtlink/verified/test/test-smtlink-hint.lisp
@@ -1,0 +1,23 @@
+(in-package "SMT")
+(include-book "std/util/define" :dir :system)
+(include-book "../hint-interface")
+
+(define foo ((x integerp)
+             (y rationalp))
+  :returns (res rationalp)
+  (b* ((x (ifix x))
+       (y (rfix y)))
+    (+ x y)))
+
+(defun smt-fun ()
+  `(,(make-smt-function
+      :name 'ifix
+      :expansion-depth 0)
+    ,(make-smt-function
+      :name 'rfix
+      :expansion-depth 0)))
+
+(defun my-hint ()
+  (make-smtlink-hint
+   :functions (smt-fun)
+   :wrld-fn-len 99))
